CertiGrad/Graph.lean
@@ -1,0 +1,212 @@
+/-
+Copyright (c) 2017 Daniel Selsam. All rights reserved.
+Released under Apache 2.0 license as described in the file LICENSE.
+Author: Daniel Selsam
+
+Stochastic computation graphs.
+-/
+-- import .det .rand .util .id .sprog .env .reference
+
+import CertiGrad.Det
+import CertiGrad.Rand
+import CertiGrad.Util
+import CertiGrad.Id
+import CertiGrad.Sprog
+import CertiGrad.Env
+import CertiGrad.Reference
+
+namespace certigrad
+
+inductive Operator (ishapes : List S) (oshape : S) : Type
+| det : det.op ishapes oshape → Operator ishapes oshape
+| rand : rand.op ishapes oshape → Operator ishapes oshape
+
+noncomputable
+def Operator.to_dist (m : Env) : ∀ {parents : List Reference} {oshape : S}, Operator parents.p2 oshape → sprog [oshape]
+| parents, _, (det op)   => sprog.ret ⟦op.f (env.get_ks parents m)⟧
+| parents, _, (rand op) => sprog.prim op (env.get_ks parents m)
+
+
+structure Node : Type where
+  ref : Reference
+  parents : List (ID × S)
+  op : Operator parents.p2 ref.2
+
+structure Graph : Type := (nodes : List Node) (costs : List ID) (targets inputs : List Reference)
+
+/-
+
+def uniq_ids : ∀ (nodes : List Node) (inputs : env), Prop
+| [], inputs => true
+| (⟨ref, op, parents⟩ :: nodes), inputs =>
+¬ env.has_key ref inputs ∧ ∀ (x : T ref.2), uniq_ids nodes (env.insert ref x inputs)
+
+namespace graph
+
+open sprog
+
+def to_dist {fshapes : List S} (k : env → dvec T fshapes) : env → List Node → sprog fshapes
+| m []            => ret (k m)
+| m (⟨ref, parents, op⟩::nodes) => bind (operator.to_dist m op)
+                                        (λ (x : dvec T [ref.2]), to_dist (env.insert ref x^.head m) nodes)
+
+open list
+
+lemma envs_match_helper {fshapes : List S} (k₁ k₂ : env → dvec T fshapes) : ∀ (inputs : env) (nodes : List Node),
+    ∀ (n : node) (x : T n^.ref.2),
+      uniq_ids (n :: nodes) inputs →
+      (∀ (m : env), (∀ (ref : Reference), env.has_key ref inputs → env.get ref m = env.get ref inputs) → k₁ m = k₂ m) →
+      ∀  (m : env),
+         (∀ (r : Reference), env.has_key r (env.insert n^.ref x inputs) → env.get r m = env.get r (env.insert n^.ref x inputs)) → k₁ m = k₂ m :=
+assume inputs nodes n x H_uids H_k_eq,
+assume (m : env) H_next_envs_agree,
+  have H_envs_agree : ∀ (ref' : Reference), env.has_key ref' inputs → env.get ref' m = env.get ref' inputs, from
+    assume (ref' : Reference) (H_inputs_contains_ref' : env.has_key ref' inputs),
+    show env.get ref' m = env.get ref' inputs, from
+    have H_next_contains_name : env.has_key ref' (env.insert n^.ref x inputs), from env.has_key_insert H_inputs_contains_ref',
+    have H_next_agree : env.get ref' m = env.get ref' (env.insert n^.ref x inputs), from H_next_envs_agree _ H_next_contains_name,
+    have H_ref'_neq_ref : ref' ≠ n^.ref,
+      begin
+      cases n with ref parents op, dsimp [uniq_ids] at H_uids,
+      dsimp, intro H_eq, subst H_eq, exact H_uids^.left H_inputs_contains_ref'
+      end,
+    begin rw env.get_insert_diff _ _ H_ref'_neq_ref at H_next_agree, exact H_next_agree end,
+  H_k_eq _ H_envs_agree
+
+lemma to_dist_k_congr {fshapes : List S} (k₁ k₂ : env → dvec T fshapes) (inputs : env) (nodes : List Node) :
+  k₁ = k₂ →  graph.to_dist k₁ inputs nodes = graph.to_dist k₂ inputs nodes := by { intro H, rw H }
+
+lemma to_dist_congr {fshapes : List S} (k₁ k₂ : env → dvec T fshapes) : ∀ (inputs : env) (nodes : List Node),
+      uniq_ids nodes inputs →
+      (∀ (m : env), (∀ (ref : Reference), env.has_key ref inputs → env.get ref m = env.get ref inputs) → k₁ m = k₂ m) →
+      to_dist k₁ inputs nodes = to_dist k₂ inputs nodes
+
+-- Case 1
+| inputs [] H_uids H_k_eq :=
+show to_dist k₁ inputs [] = to_dist k₂ inputs [], from
+show sprog.ret (k₁ inputs) = sprog.ret (k₂ inputs), from
+have H_inputs_eq : ∀ (ref : Reference), env.has_key ref inputs → env.get ref inputs = env.get ref inputs, from
+  assume (ref : Reference) (H_inputs_contain : env.has_key ref inputs), rfl,
+by rw (H_k_eq _ H_inputs_eq)
+
+-- Case 2
+| inputs (⟨ref, parents, op⟩::nodes) H_uids H_k_eq :=
+show to_dist k₁ inputs (⟨ref, parents, op⟩ :: nodes) = to_dist k₂ inputs (⟨ref, parents, op⟩ :: nodes), from
+show bind (operator.to_dist inputs op) (λ (x : dvec T [ref.2]), to_dist k₁ (env.insert ref x^.head inputs) nodes)
+     =
+     bind (operator.to_dist inputs op) (λ (x : dvec T [ref.2]), to_dist k₂ (env.insert ref x^.head inputs) nodes), from
+suffices ∀ (x : dvec T [ref.2]), to_dist k₁ (env.insert ref x^.head inputs) nodes = to_dist k₂ (env.insert ref x^.head inputs) nodes, from
+  congr_arg _ (funext this),
+assume (x : dvec T [ref.2]),
+show to_dist k₁ (env.insert ref x^.head inputs) nodes = to_dist k₂ (env.insert ref x^.head inputs) nodes, from
+to_dist_congr _ _ (H_uids^.right _) (envs_match_helper k₁ k₂ _ _ _ _ H_uids H_k_eq)
+
+lemma graph_to_dist_inputs_congr {fshapes : List S} (k : env → dvec T fshapes) (inputs₁ inputs₂ : env) (nodes : List Node) :
+  inputs₁ = inputs₂ → graph.to_dist k inputs₁ nodes = graph.to_dist k inputs₂ nodes := assume H, by rw H
+
+end graph
+
+noncomputable def is_gintegrable {shapes : List S} (k : env → dvec T shapes) {shape : S} : ∀ (m : env) (nodes : List Node) (f : dvec T shapes → T shape), Prop
+| _ [] f => true
+
+| m (⟨ref, parents, operator.det op⟩ :: nodes) f => is_gintegrable (env.insert ref (op^.f (env.get_ks parents m)) m) nodes f
+
+| m (⟨ref, parents, operator.rand op⟩ :: nodes) f :=
+  let m' := (λ (y : T ref.2), env.insert ref y m) in
+  T.is_integrable (λ x, op^.pdf (env.get_ks parents m) x ⬝ E (graph.to_dist k (m' x) nodes) f) ∧
+  ∀ x, is_gintegrable (m' x) nodes f
+
+open list
+
+noncomputable def is_gdifferentiable (k : env → dvec T [[]]) : ∀ (tgt : Reference) (m : env) (nodes : List Node) (f : dvec T [[]] → ℝ), Prop
+| tgt _ [] f := true
+
+| tgt m (⟨ref, parents, operator.det op⟩ :: nodes) f :=
+let θ := env.get tgt m,
+    x := op^.f (env.get_ks parents m),
+    g := (λ (v : dvec T parents^.p2) (θ : T tgt.2), E (graph.to_dist k (env.insert ref (det.op.f op v) (env.insert tgt θ m)) nodes) dvec.head) in
+
+T.is_cdifferentiable (λ (θ₀ : T (tgt.snd)), g (env.get_ks parents (env.insert tgt θ m)) θ₀) θ
+∧ T.is_cdifferentiable (λ (θ₀ : T (tgt.snd)), sumr (map (λ (idx : ℕ), g (dvec.update_at θ₀ (env.get_ks parents (env.insert tgt θ m)) idx) θ)
+                                                       (filter (λ (idx : ℕ), tgt = dnth parents idx) (riota (length parents))))) θ
+∧ is_gdifferentiable tgt (env.insert ref x m) nodes f
+∧ ∀ {idx : ℕ}, idx ∈ riota (length parents) → tgt = dnth parents idx → is_gdifferentiable ref (env.insert ref x m) nodes f
+
+| tgt m (⟨ref, parents, operator.rand op⟩ :: nodes) f :=
+let g : dvec T [ref.2] → T tgt.2 → ℝ :=
+           (λ (x : dvec T [ref.2]) (θ₀ : T tgt.2), E (graph.to_dist k (env.insert ref x^.head (env.insert tgt θ₀ m)) nodes) dvec.head),
+   θ : T tgt.2 := env.get tgt m,
+   m' := (λ (y : T ref.2), env.insert ref y m) in
+
+T.is_cdifferentiable (λ (θ₀ : T (tgt.snd)), E (sprog.prim op (env.get_ks parents (env.insert tgt θ m))) (λ (y : dvec T [ref.snd]), g y θ₀)) θ
+∧ T.is_cdifferentiable (λ (θ₀ : T (tgt.snd)), sumr (map (λ (idx : ℕ), E (sprog.prim op (dvec.update_at θ₀ (env.get_ks parents (env.insert tgt θ m)) idx))
+                                                                       (λ (y : dvec T [ref.snd]), g y θ))
+                                                       (filter (λ (idx : ℕ), tgt = dnth parents idx) (riota (length parents))))) θ
+∧ ∀ (y : T ref.2), is_gdifferentiable tgt (env.insert ref y m) nodes f
+
+lemma is_gintegrable_k_congr {fshapes : List S} {fshape : S} (k₁ k₂ : env → dvec T fshapes) : ∀ (inputs : env) (nodes : List Node) (f : dvec T fshapes → T fshape),
+  uniq_ids nodes inputs →
+  (∀ (m : env), (∀ (ref : Reference), env.has_key ref inputs → env.get ref m = env.get ref inputs) → k₁ m = k₂ m) →
+  is_gintegrable k₁ inputs nodes f → is_gintegrable k₂ inputs nodes f
+
+| inputs [] f H_uids H_k_eq H_gint₁ => trivial
+
+| inputs (⟨ref, parents, operator.det op⟩ :: nodes) f H_uids H_k_eq H_gint₁ :=
+begin
+dsimp [is_gintegrable] at H_gint₁,
+dsimp [is_gintegrable],
+apply is_gintegrable_k_congr _ _ _ (H_uids^.right _) (graph.envs_match_helper k₁ k₂ _ _ _ _ H_uids H_k_eq) H_gint₁
+end
+
+| inputs (⟨ref, parents, operator.rand op⟩ :: nodes) f H_uids H_k_eq H_gint₁ :=
+begin
+dsimp [is_gintegrable] at H_gint₁,
+dsimp [is_gintegrable],
+split,
+{
+assertv H_dist_congr : ∀ x, graph.to_dist k₁ (env.insert ref x inputs) nodes = graph.to_dist k₂ (env.insert ref x inputs) nodes :=
+assume x,
+graph.to_dist_congr k₁ k₂ _ _ (H_uids^.right _) (graph.envs_match_helper k₁ k₂ _ _ _ _ H_uids H_k_eq),
+simp only [H_dist_congr] at H_gint₁,
+exact H_gint₁^.left
+},
+
+{
+intro x,
+apply is_gintegrable_k_congr _ _ _ (H_uids^.right _) (graph.envs_match_helper k₁ k₂ _ _ _ _ H_uids H_k_eq) (H_gint₁^.right x)
+}
+
+end
+
+-- TODO(dhs): this seems like it could be provable given is_gintegrable and compute_grad_slow_correct
+noncomputable def is_nabla_gintegrable (k : env → dvec T [[]]) : ∀ (tgt : Reference) (m : env) (nodes : List Node) (f : dvec T [[]] → ℝ), Prop
+| tgt m [] f => true
+
+| tgt m (⟨ref, parents, operator.det op⟩ :: nodes) f :=
+  is_nabla_gintegrable tgt (env.insert ref (op^.f (env.get_ks parents m)) m) nodes f
+  ∧ ∀ {idx : ℕ}, idx ∈ riota (length parents) → tgt = dnth parents idx → is_nabla_gintegrable ref (env.insert ref (op^.f (env.get_ks parents m)) m) nodes f
+
+| tgt m (⟨ref, parents, operator.rand op⟩ :: nodes) f :=
+  T.is_integrable (λ (x : T ref.2), op^.pdf (env.get_ks parents m) x ⬝ ∇ (λ (θ₀ : T tgt.2), E (graph.to_dist k (env.insert ref x (env.insert tgt θ₀ m)) nodes) f) (env.get tgt m))
+
+∧ T.is_integrable
+    (λ (x : T (ref.snd)),
+       rand.op.pdf op (env.get_ks parents m) x ⬝ sumr
+         (map
+            (λ (idx : ℕ),
+               E
+                 (graph.to_dist k
+                    (env.insert ref x m)
+                    nodes)
+                 dvec.head ⬝ ∇
+                 (λ (θ₀ : T (tgt.snd)),
+                    T.log (rand.op.pdf op (dvec.update_at θ₀ (env.get_ks parents m) idx) x))
+                 (env.get tgt m))
+            (filter (λ (idx : ℕ), tgt = dnth parents idx) (riota (length parents)))))
+
+  ∧ ∀ (y : T ref.2), is_nabla_gintegrable tgt (env.insert ref y m) nodes f
+
+--  is_gintegrable (λ m, ⟦compute_grad_slow costs nodes m tgt⟧) inputs nodes dvec.head →
+
+-/
+end certigrad
