CertiGrad/Program.lean
@@ -1,0 +1,250 @@
+/-
+Copyright (c) 2017 Daniel Selsam. All rights reserved.
+Released under Apache 2.0 license as described in the file LICENSE.
+Author: Daniel Selsam
+
+A Term language for conveniently constructing stochastic computation graphs.
+-/
+-- import .tensor .graph .tactics .ops data.hash_map
+
+import CertiGrad.Tensor
+import CertiGrad.Graph
+import CertiGrad.Ops
+import CertiGrad.Tactics
+
+
+#print "compiling program..."
+
+namespace certigrad
+namespace program
+
+-- open list
+
+inductive UnaryOp : Type
+| neg : UnaryOp
+| exp : UnaryOp
+| log : UnaryOp
+| sqrt : UnaryOp
+| softplus : UnaryOp
+| sigmoid : UnaryOp
+
+inductive BinaryOp : Type
+| add : BinaryOp
+| sub : BinaryOp
+| mul : BinaryOp
+| div : BinaryOp
+
+inductive Term : Type
+| unary : UnaryOp → Term → Term
+| binary : BinaryOp → Term → Term → Term
+| sum : Term → Term
+| scale : TReal→ Term → Term
+| gemm : Term → Term → Term
+| mvn_kl : Term → Term → Term
+| mvn_empirical_kl : Term → Term → Term → Term
+| bernoulli_neglogpdf : Term → Term → Term
+| id : label → Term
+
+-- instance : has_neg Term := ⟨term.unary UnaryOp.neg⟩
+-- instance : has_smul TRealterm := ⟨term.scale⟩
+-- instance : has_add Term := ⟨term.binary BinaryOp.add⟩
+-- instance : has_sub Term := ⟨term.binary BinaryOp.sub⟩
+-- instance : has_mul Term := ⟨term.binary BinaryOp.mul⟩
+-- instance : has_div Term := ⟨term.binary BinaryOp.div⟩
+
+-- instance coe_id : has_coe label Term := ⟨term.id⟩
+
+def exp : Term → Term := Term.unary UnaryOp.exp
+def log : Term → Term := Term.unary UnaryOp.log
+def sqrt : Term → Term := Term.unary UnaryOp.sqrt
+def softplus : Term → Term := Term.unary UnaryOp.softplus
+def sigmoid : Term → Term := Term.unary UnaryOp.sigmoid
+
+inductive rterm : Type
+| mvn : Term → Term → rterm
+| mvn_std : S → rterm
+
+inductive statement : Type
+| param : label → S → statement
+| input : label → S → statement
+| cost : label → statement
+| assign : label → Term → statement
+| sample : label → rterm → statement
+
+-- structure state : Type :=
+--   (next_id : ℕ) (shapes : hash_map label (λ x => S))
+--   (nodes : List node) (costs : List ID) (targets inputs : List Reference)
+
+-- def empty_state : state := ⟨0, mk_hash_map (λ (x : label)=> x^.to_nat), [], [], [], []⟩
+
+-- operators like `ops.neg` are currently commented out in `Ops.lean`
+-- def unary_to_op (shape : S) : UnaryOp → det.op [shape] shape
+-- | UnaryOp.neg      => ops.neg shape
+-- | UnaryOp.exp      => ops.exp shape
+-- | UnaryOp.log      => ops.log shape
+-- | UnaryOp.sqrt     => ops.sqrt shape
+-- | UnaryOp.softplus => ops.softplus shape
+-- | UnaryOp.sigmoid  => ops.sigmoid shape
+
+-- def binary_to_op (shape : S) : BinaryOp → det.op [shape, shape] shape
+-- | BinaryOp.add     => ops.add shape
+-- | BinaryOp.mul     => ops.mul shape
+-- | BinaryOp.sub     => ops.sub shape
+-- | BinaryOp.div     => ops.div shape
+
+def get_id (next_id : ℕ) : Option ID → ID
+| none => ID.nat next_id
+| (some ident) => ident
+
+/-
+def process_term : Term → state → Option ID → Reference × state
+
+| (term.unary f t) st ident :=
+    match process_term t st none with
+    | ((p₁, shape), ⟨next_id, shapes, nodes, costs, targets, inputs⟩) :=
+      ((ID.nat $ next_id, shape),
+        ⟨next_id+1, shapes,
+         concat nodes ⟨(get_id next_id ident, shape), [(p₁, shape)], operator.det (unary_to_op shape f)⟩,
+         costs, targets, inputs⟩)
+    end
+
+| (term.binary f t₁ t₂) st ident :=
+    match process_term t₁ st none with
+    | ((p₁, shape'), st') :=
+    match process_term t₂ st' none with
+    | ((p₂, shape), ⟨next_id, shapes, nodes, costs, targets, inputs⟩) :=
+      ((get_id next_id ident, shape),
+       ⟨next_id+1, shapes,
+        concat nodes ⟨(get_id next_id ident, shape), [(p₁, shape), (p₂, shape)], operator.det (binary_to_op shape f)⟩,
+               costs, targets, inputs⟩)
+    end
+    end
+
+| (term.sum t) st ident :=
+    match process_term t st none with
+    | ((p₁, shape), ⟨next_id, shapes, nodes, costs, targets, inputs⟩) :=
+      ((get_id next_id ident, []),
+        ⟨next_id+1, shapes,
+         concat nodes ⟨(get_id next_id ident, []), [(p₁, shape)], operator.det (ops.sum shape)⟩,
+         costs, targets, inputs⟩)
+    end
+
+| (term.scale α t) st ident :=
+    match process_term t st none with
+    | ((p₁, shape), ⟨next_id, shapes, nodes, costs, targets, inputs⟩) :=
+      ((get_id next_id ident, shape),
+       ⟨next_id+1, shapes,
+       concat nodes ⟨(get_id next_id ident, shape), [(p₁, shape)], operator.det (ops.scale α shape)⟩,
+       costs, targets, inputs⟩)
+    end
+
+| (term.gemm t₁ t₂) st ident :=
+    match process_term t₁ st none with
+    | ((p₁, shape₁), st') :=
+    match process_term t₂ st' none with
+    | ((p₂, shape₂), ⟨next_id, shapes, nodes, costs, targets, inputs⟩) :=
+      let m := shape₁.head, n := shape₂.head, p := shape₂.tail.head in
+      ((get_id next_id ident, [m, p]),
+       ⟨next_id+1, shapes,
+        concat nodes ⟨(get_id next_id ident, [m, p]), [(p₁, [m, n]), (p₂, [n, p])], operator.det (ops.gemm _ _ _)⟩,
+        costs, targets, inputs⟩)
+    end
+    end
+
+| (term.mvn_kl t₁ t₂) st ident :=
+    match process_term t₁ st none with
+    | ((p₁, shape'), st') :=
+    match process_term t₂ st' none with
+    | ((p₂, shape), ⟨next_id, shapes, nodes, costs, targets, inputs⟩) :=
+      ((get_id next_id ident, []), ⟨next_id+1, shapes,
+        concat nodes ⟨(get_id next_id ident, []), [(p₁, shape), (p₂, shape)], operator.det (ops.mvn_kl shape)⟩,
+        costs, targets, inputs⟩)
+    end
+    end
+
+| (term.mvn_empirical_kl t₁ t₂ t₃) st ident :=
+    match process_term t₁ st none with
+    | ((p₁, shape''), st') :=
+    match process_term t₂ st' none with
+    | ((p₂, shape'), st'') :=
+    match process_term t₃ st'' none with
+    | ((p₃, shape), ⟨next_id, shapes, nodes, costs, targets, inputs⟩) :=
+      ((get_id next_id ident, []), ⟨next_id+1, shapes,
+        concat nodes ⟨(get_id next_id ident, []), [(p₁, shape), (p₂, shape), (p₃, shape)], operator.det (det.op.mvn_empirical_kl shape)⟩,
+        costs, targets, inputs⟩)
+    end
+    end
+    end
+
+| (term.bernoulli_neglogpdf t₁ t₂) st ident :=
+    match process_term t₁ st none with
+    | ((p₁, shape'), st') :=
+    match process_term t₂ st' none with
+    | ((p₂, shape), ⟨next_id, shapes, nodes, costs, targets, inputs⟩) :=
+      ((get_id next_id ident, []),
+        ⟨next_id+1, shapes,
+         concat nodes ⟨(get_id next_id ident, []), [(p₁, shape), (p₂, shape)], operator.det (ops.bernoulli_neglogpdf shape)⟩,
+         costs, targets, inputs⟩)
+    end
+    end
+
+| (term.id s) ⟨next_id, shapes, nodes, costs, targets, inputs⟩ ident :=
+   match shapes^.find s with
+   | (some shape) := ((ID.str s, shape), ⟨next_id, shapes, nodes, costs, targets, inputs⟩)
+   | none         := (default _, empty_state)
+   end
+
+def process_rterm : rterm → state → Option ID → Reference × state
+| (rterm.mvn t₁ t₂) st ident :=
+    match process_term t₁ st none with
+    | ((p₁, shape'), st') :=
+    match process_term t₂ st' none with
+    | ((p₂, shape), ⟨next_id, shapes, nodes, costs, targets, inputs⟩) :=
+      ((get_id next_id ident, shape),
+        ⟨next_id+1, shapes,
+         concat nodes ⟨(get_id next_id ident, shape), [(p₁, shape), (p₂, shape)], operator.rand (rand.op.mvn shape)⟩,
+         costs, targets, inputs⟩)
+    end
+    end
+
+| (rterm.mvn_std shape) ⟨next_id, shapes, nodes, costs, targets, inputs⟩ ident :=
+  ((get_id next_id ident, shape),
+   ⟨next_id+1, shapes,
+    nodes ++ [⟨(get_id next_id ident, shape), [], operator.rand (rand.op.mvn_std shape)⟩],
+    costs, targets, inputs⟩)
+
+def program_to_graph_core : List statement → state → state
+| [] st := st
+
+| (statement.assign s t::statements) st :=
+  match process_term t st (some (ID.str s)) with
+  | ((_, shape), ⟨next_id, shapes, nodes, costs, targets, inputs⟩) :=
+     program_to_graph_core statements ⟨next_id, shapes^.insert s shape, nodes, costs, targets, inputs⟩
+  end
+
+| (statement.sample s t::statements) st :=
+  match process_rterm t st (some (ID.str s)) with
+  | ((_, shape), ⟨next_id, shapes, nodes, costs, targets, inputs⟩) :=
+    program_to_graph_core statements ⟨next_id, shapes^.insert s shape, nodes, costs, targets, inputs⟩
+  end
+
+| (statement.param s shape::statements) ⟨next_id, shapes, nodes, costs, targets, inputs⟩ :=
+  program_to_graph_core statements ⟨next_id, shapes^.insert s shape, nodes, costs, concat targets (ID.str s, shape), concat inputs (ID.str s, shape)⟩
+| (statement.input s shape::statements) ⟨next_id, shapes, nodes, costs, targets, inputs⟩ :=
+  program_to_graph_core statements ⟨next_id, shapes^.insert s shape, nodes, costs, targets, concat inputs (ID.str s, shape)⟩
+| (statement.cost s::statements) ⟨next_id, shapes, nodes, costs, targets, inputs⟩ :=
+  program_to_graph_core statements ⟨next_id, shapes, nodes, concat costs (ID.str s), targets, inputs⟩
+-/
+end program
+
+def program := List program.statement
+
+-- def program_to_graph : program → graph
+-- | prog =>  match program.program_to_graph_core prog program.empty_state with
+--            | ⟨next_id, shapes, nodes, costs, targets, inputs⟩ => ⟨nodes, costs, targets, inputs⟩
+--            end
+
+-- def mk_inputs : ∀ (g : graph), Dvec T g.inputs.p2 → env
+-- | g, ws => env.insert_all g.inputs ws
+
+end certigrad
